added most simulations

systems/SerializedSimulations.v
@@ -16,7 +16,7 @@ Section SerializedCorrect.
   Context {orig_msg_serializer : Serializer msg}.
 
   Instance orig_multi_params_name_tot_map :
-    MultiParamsNameTotalMap orig_multi_params multi_params :=
+    MultiParamsNameTotalMap orig_multi_params serialized_multi_params :=
   {
     tot_map_name := id ;
     tot_map_name_inv := id
@@ -30,7 +30,7 @@ Section SerializedCorrect.
   }.
 
   Instance orig_base_params_tot_map :
-    BaseParamsTotalMap orig_base_params base_params :=
+    BaseParamsTotalMap orig_base_params serialized_base_params :=
   {
     tot_map_data := id;
     tot_map_input := serialize;
@@ -38,12 +38,12 @@ Section SerializedCorrect.
   }.
 
   Instance orig_multi_params_tot_msg_map :
-    MultiParamsMsgTotalMap orig_multi_params multi_params :=
+    MultiParamsMsgTotalMap orig_multi_params serialized_multi_params :=
   {
     tot_map_msg := serialize
   }.
 
-  Instance refined_multi_params_map_congruency :
+  Instance orig_multi_params_map_congruency :
     MultiParamsTotalMapCongruency orig_base_params_tot_map
       orig_multi_params_name_tot_map orig_multi_params_tot_msg_map :=
   {
@@ -89,16 +89,16 @@ Section SerializedCorrect.
   Qed.
 
   Definition serialize_packet p :=
-    @mkPacket _ multi_params
+    @mkPacket _ serialized_multi_params
               (@pSrc _ orig_multi_params p)
               (pDst p)
               (serialize (pBody p)).
 
-  Definition serialize_net (net : @network _ orig_multi_params) : (@network _ multi_params) :=
-    @mkNetwork _ multi_params (map serialize_packet (nwPackets net)) net.(nwState).
+  Definition serialize_net (net : @network _ orig_multi_params) : (@network _ serialized_multi_params) :=
+    @mkNetwork _ serialized_multi_params (map serialize_packet (nwPackets net)) net.(nwState).
 
   Definition serialize_tr_entry (e : @name _ orig_multi_params * (@input orig_base_params + list (@output orig_base_params))) : 
-  @name _ multi_params * (@input base_params + list (@output base_params)) := 
+  @name _ serialized_multi_params * (@input serialized_base_params + list (@output serialized_base_params)) := 
   let (n, s) := e in
   match s with
   | inl io => (n, inl (serialize io))
@@ -108,7 +108,7 @@ Section SerializedCorrect.
   Theorem step_async_serialize_simulation_1 :
     forall net net' tr,
       @step_async _ orig_multi_params net net' tr ->
-      @step_async _ multi_params (serialize_net net) (serialize_net net') (map serialize_tr_entry tr).
+      @step_async _ serialized_multi_params (serialize_net net) (serialize_net net') (map serialize_tr_entry tr).
   Proof.
   move => net net' out H_step.
   apply step_async_tot_mapped_simulation_1 in H_step.
@@ -125,7 +125,7 @@ Section SerializedCorrect.
   Lemma step_async_serialize_simulation_star_1 :
     forall net tr,
       @step_async_star _ orig_multi_params step_async_init net tr ->
-      @step_async_star _ multi_params step_async_init (serialize_net net) (map serialize_tr_entry tr).
+      @step_async_star _ serialized_multi_params step_async_init (serialize_net net) (map serialize_tr_entry tr).
   Proof.
   move => net tr H_step.
   apply step_async_tot_mapped_simulation_star_1 in H_step.
@@ -139,17 +139,17 @@ Section SerializedCorrect.
   by rewrite H_eq {H_eq fp}. 
   Qed.
 
-  Definition deserialize_packet (p : @packet _ multi_params) : option (@packet _ orig_multi_params) :=
+  Definition deserialize_packet (p : @packet _ serialized_multi_params) : option (@packet _ orig_multi_params) :=
     match (deserialize (pBody p)) with
     | None => None
     | Some (body, _) =>
       Some (@mkPacket _ orig_multi_params (pSrc p) (pDst p) body)
     end.
 
-  Definition deserialize_net (net: @network _ multi_params) :  (@network _ orig_multi_params) :=
+  Definition deserialize_net (net: @network _ serialized_multi_params) :  (@network _ orig_multi_params) :=
     mkNetwork (filterMap deserialize_packet (nwPackets net)) net.(nwState).
 
-  Definition deserialize_tr_entry (e : @name _ multi_params * (@input base_params + list (@output base_params))) :
+  Definition deserialize_tr_entry (e : @name _ serialized_multi_params * (@input serialized_base_params + list (@output serialized_base_params))) :
     option (@name _ orig_multi_params * (@input orig_base_params + list (@output orig_base_params))) :=
   let (n, s) := e in
   match s with
@@ -195,7 +195,7 @@ Section SerializedCorrect.
   Qed.
 
   Instance multi_params_orig_name_tot_map :
-    MultiParamsNameTotalMap multi_params orig_multi_params :=
+    MultiParamsNameTotalMap serialized_multi_params orig_multi_params :=
   {
     tot_map_name := id ;
     tot_map_name_inv := id
@@ -208,7 +208,7 @@ Section SerializedCorrect.
     tot_map_name_inverse_inv := fun _ => eq_refl
   }.
 
-  Instance multi_orig_params_pt_msg_map : MultiParamsMsgPartialMap multi_params orig_multi_params :=
+  Instance multi_orig_params_pt_msg_map : MultiParamsMsgPartialMap serialized_multi_params orig_multi_params :=
   {
     pt_map_msg := fun m => 
       match deserialize m with 
@@ -217,7 +217,7 @@ Section SerializedCorrect.
       end   
   }.
 
-  Instance multi_orig_base_params_pt_map : BaseParamsPartialMap base_params orig_base_params :=
+  Instance multi_orig_base_params_pt_map : BaseParamsPartialMap serialized_base_params orig_base_params :=
   {
     pt_map_data := id;
     pt_map_input := fun i =>
@@ -355,7 +355,7 @@ Section SerializedCorrect.
 
   Theorem step_async_pt_mapped_simulation_1 :
   forall net net' tr,
-    @step_async _ multi_params net net' tr ->
+    @step_async _ serialized_multi_params net net' tr ->
     @step_async _ orig_multi_params (deserialize_net net) (deserialize_net net') (filterMap deserialize_tr_entry tr) \/ 
     (deserialize_net net' = deserialize_net net /\ pt_trace_remove_empty_out (filterMap deserialize_tr_entry tr) = []).
   Proof.
@@ -366,7 +366,7 @@ Section SerializedCorrect.
 
   Lemma step_async_pt_mapped_simulation_star_1 :
   forall net tr,
-    @step_async_star _ multi_params step_async_init net tr ->
+    @step_async_star _ serialized_multi_params step_async_init net tr ->
     exists tr', @step_async_star _ orig_multi_params step_async_init (deserialize_net net) tr' /\ 
      pt_trace_remove_empty_out (filterMap deserialize_tr_entry tr) = pt_trace_remove_empty_out tr'.
   Proof.
@@ -376,6 +376,151 @@ Section SerializedCorrect.
   break_and.
   exists x.
   by rewrite -pt_map_trace_filterMap -pt_map_net_deserialize_net.
+  Qed.
+
+  Context {orig_name_overlay_params : NameOverlayParams orig_multi_params}.
+  Context {orig_fail_msg_params : FailMsgParams orig_multi_params}.
+
+  Instance multi_orig_fail_msg_params_pt_map_congruency : FailMsgParamsPartialMapCongruency serialized_fail_msg_params orig_fail_msg_params multi_orig_params_pt_msg_map :=
+  {
+    pt_fail_msg_fst_snd := _
+  }.
+  Proof.
+  rewrite /pt_map_msg /=.
+  by rewrite serialize_deserialize_id_nil.
+  Qed.
+
+  Instance multi_orig_name_overlay_params_tot_map_congruency : NameOverlayParamsTotalMapCongruency serialized_name_overlay_params orig_name_overlay_params multi_params_orig_name_tot_map := 
+  {
+    tot_adjacent_to_fst_snd := fun _ _ => conj (fun H => H) (fun H => H)
+  }.
+
+  Lemma step_ordered_failure_pt_mapped_simulation_1 :
+  forall net net' failed failed' tr,
+    @step_ordered_failure _ _ serialized_name_overlay_params serialized_fail_msg_params (failed, net) (failed', net') tr ->
+    @step_ordered_failure _ _ orig_name_overlay_params orig_fail_msg_params (failed, pt_map_onet net) (failed', pt_map_onet net') (pt_map_traces tr) \/
+    pt_map_onet net = pt_map_onet net' /\ failed = failed' /\ pt_map_traces tr = [].
+  Proof.
+  move => net net' failed failed' tr H_st.
+  eapply step_ordered_failure_pt_mapped_simulation_1 in H_st.
+  case: H_st => H_st; last by right; break_and.
+  have H_eq_n: failed = map (@tot_map_name _ _ _ _ multi_params_orig_name_tot_map) failed by rewrite /tot_map_name /= map_id.
+  rewrite {1}H_eq_n.
+  have H_eq_n': failed' = map (@tot_map_name _ _ _ _ multi_params_orig_name_tot_map) failed' by rewrite /tot_map_name /= map_id.
+  rewrite {1}H_eq_n'.
+  left.
+  exact: H_st.
+  Qed.
+
+  Theorem step_ordered_failure_pt_mapped_simulation_star_1 :
+    forall net failed tr,
+    @step_ordered_failure_star _ _ serialized_name_overlay_params serialized_fail_msg_params step_ordered_failure_init (failed, net) tr ->
+    @step_ordered_failure_star _ _ orig_name_overlay_params orig_fail_msg_params step_ordered_failure_init (failed, pt_map_onet net) (pt_map_traces tr).
+  Proof.
+  move => onet failed tr H_st.
+  apply step_ordered_failure_pt_mapped_simulation_star_1 in H_st.
+  by rewrite map_id in H_st.
+  Qed.
+    
+  Context {orig_new_msg_params : NewMsgParams orig_multi_params}.
+
+  Instance multi_orig_new_msg_params_pt_map_congruency : NewMsgParamsPartialMapCongruency serialized_new_msg_params orig_new_msg_params multi_orig_params_pt_msg_map :=
+  {
+    pt_new_msg_fst_snd := _
+  }.
+  Proof.
+  rewrite /pt_map_msg /=.
+  by rewrite serialize_deserialize_id_nil.
+  Qed.
+
+  Lemma step_ordered_dyanamic_failure_pt_mapped_simulation_1 :
+  forall net net' failed failed' tr,
+    NoDup (odnwNodes net) ->
+    @step_ordered_dynamic_failure _ _ serialized_name_overlay_params serialized_new_msg_params serialized_fail_msg_params (failed, net) (failed', net') tr ->
+    @step_ordered_dynamic_failure _ _ orig_name_overlay_params orig_new_msg_params orig_fail_msg_params (failed, pt_map_odnet net) (failed', pt_map_odnet net') (pt_map_traces tr) \/
+    pt_map_odnet net = pt_map_odnet net' /\ failed = failed' /\ pt_map_traces tr = [].
+  Proof.
+  move => net net' failed failed' tr H_nd H_st.
+  eapply step_ordered_dynamic_failure_pt_mapped_simulation_1 in H_st; last by [].
+  case: H_st => H_st; last by right; break_and.
+  have H_eq_n: failed = map (@tot_map_name _ _ _ _ multi_params_orig_name_tot_map) failed by rewrite /tot_map_name /= map_id.
+  rewrite {1}H_eq_n.
+  have H_eq_n': failed' = map (@tot_map_name _ _ _ _ multi_params_orig_name_tot_map) failed' by rewrite /tot_map_name /= map_id.
+  rewrite {1}H_eq_n'.
+  left.
+  exact: H_st.
+  Qed.
+
+  Theorem step_ordered_dynamic_failure_pt_mapped_simulation_star_1 :
+    forall net failed tr,
+    @step_ordered_dynamic_failure_star _ _ serialized_name_overlay_params serialized_new_msg_params serialized_fail_msg_params step_ordered_dynamic_failure_init (failed, net) tr ->
+    @step_ordered_dynamic_failure_star _ _ orig_name_overlay_params orig_new_msg_params orig_fail_msg_params step_ordered_dynamic_failure_init (failed, pt_map_odnet net) (pt_map_traces tr).
+  Proof.
+  move => onet failed tr H_st.
+  apply step_ordered_dynamic_failure_pt_mapped_simulation_star_1 in H_st.
+  by rewrite map_id in H_st.
+  Qed.
+
+  Instance orig_multi_fail_msg_params_tot_map_congruency : FailMsgParamsTotalMapCongruency orig_fail_msg_params serialized_fail_msg_params orig_multi_params_tot_msg_map :=
+  {
+    tot_fail_msg_fst_snd := eq_refl
+  }.
+
+  Instance orig_multi_name_overlay_params_tot_map_congruency : NameOverlayParamsTotalMapCongruency orig_name_overlay_params serialized_name_overlay_params orig_multi_params_name_tot_map := 
+  {
+    tot_adjacent_to_fst_snd := fun _ _ => conj (fun H => H) (fun H => H)
+  }.
+
+  Lemma step_ordered_failure_tot_mapped_simulation_1 :
+  forall net net' failed failed' tr,
+    @step_ordered_failure _ _ orig_name_overlay_params orig_fail_msg_params (failed, net) (failed', net') tr ->
+    @step_ordered_failure _ _ serialized_name_overlay_params serialized_fail_msg_params (failed, tot_map_onet net) (failed', tot_map_onet net') (map tot_map_trace tr).
+  Proof.
+  move => net net' failed failed' tr H_step.
+  have H_st := @step_ordered_failure_tot_mapped_simulation_1 _ _ _ _ _ _ _ orig_multi_params_name_tot_map_bijective orig_multi_params_map_congruency _ _ orig_multi_name_overlay_params_tot_map_congruency _ _ orig_multi_fail_msg_params_tot_map_congruency _ _ _ _ _ H_step.
+  have H_eq_n: failed = map (@tot_map_name _ _ _ _ orig_multi_params_name_tot_map) failed by rewrite /tot_map_name /= map_id.
+  rewrite {1}H_eq_n.
+  have H_eq_n': failed' = map (@tot_map_name _ _ _ _ orig_multi_params_name_tot_map) failed' by rewrite /tot_map_name /= map_id.
+  rewrite {1}H_eq_n'.
+  apply: H_st.
+  Qed.
+
+  Lemma step_ordered_failure_tot_mapped_simulation_star_1 :
+  forall net failed tr,
+    @step_ordered_failure_star _ _ orig_name_overlay_params orig_fail_msg_params step_ordered_failure_init (failed, net) tr ->
+    @step_ordered_failure_star _ _ serialized_name_overlay_params serialized_fail_msg_params step_ordered_failure_init (map tot_map_name failed, tot_map_onet net) (map tot_map_trace tr).
+  Proof.
+  move => net failed tr.
+  exact: step_ordered_failure_tot_mapped_simulation_star_1.
+  Qed.
+  
+  Instance orig_multi_new_msg_params_tot_map_congruency : NewMsgParamsTotalMapCongruency orig_new_msg_params serialized_new_msg_params orig_multi_params_tot_msg_map :=
+  {
+    tot_new_msg_fst_snd := eq_refl
+  }.
+
+  Lemma step_ordered_dynamic_failure_tot_mapped_simulation_1 :
+  forall net net' failed failed' tr,
+    NoDup (odnwNodes net) ->
+    @step_ordered_dynamic_failure _ _ orig_name_overlay_params orig_new_msg_params orig_fail_msg_params (failed, net) (failed', net') tr ->
+    @step_ordered_dynamic_failure _ _ serialized_name_overlay_params serialized_new_msg_params serialized_fail_msg_params (failed, tot_map_odnet net) (failed', tot_map_odnet net') (map tot_map_trace tr).
+  Proof.
+  move => net net' failed failed' tr H_nd H_step.
+  have H_st := @step_ordered_dynamic_failure_tot_mapped_simulation_1 _ _ _ _ _ _ _ orig_multi_params_name_tot_map_bijective orig_multi_params_map_congruency _ _ orig_multi_name_overlay_params_tot_map_congruency _ _ orig_multi_fail_msg_params_tot_map_congruency _ _ orig_multi_new_msg_params_tot_map_congruency _ _ _ _ _ H_nd H_step.
+  have H_eq_n: failed = map (@tot_map_name _ _ _ _ orig_multi_params_name_tot_map) failed by rewrite /tot_map_name /= map_id.
+  rewrite {1}H_eq_n.
+  have H_eq_n': failed' = map (@tot_map_name _ _ _ _ orig_multi_params_name_tot_map) failed' by rewrite /tot_map_name /= map_id.
+  rewrite {1}H_eq_n'.
+  exact: H_st.
+  Qed.
+
+  Lemma step_ordered_dynamic_failure_tot_mapped_simulation_star_1 :
+  forall net failed tr,
+    @step_ordered_dynamic_failure_star _ _ orig_name_overlay_params orig_new_msg_params orig_fail_msg_params step_ordered_dynamic_failure_init (failed, net) tr ->
+    @step_ordered_dynamic_failure_star _ _ serialized_name_overlay_params serialized_new_msg_params serialized_fail_msg_params step_ordered_dynamic_failure_init (map tot_map_name failed, tot_map_odnet net) (map tot_map_trace tr).
+  Proof.
+  move => net failed tr.
+  exact: step_ordered_dynamic_failure_tot_mapped_simulation_star_1.
   Qed.
 
 End SerializedCorrect.
