systems/Serialized.v
@@ -44,14 +44,14 @@ Section Serialized.
       serialize_handler_result (input_handlers h inp d)
     end.
 
-  Instance base_params : BaseParams :=
+  Instance serialized_base_params : BaseParams :=
     {
       data := data;
       input := list bool;
       output := list bool
     }.
 
-  Instance multi_params : MultiParams _ :=
+  Instance serialized_multi_params : MultiParams _ :=
     {
       name := name;
       name_eq_dec := name_eq_dec;
@@ -66,7 +66,39 @@ Section Serialized.
     - eauto using all_names_nodes.
     - eauto using no_dup_nodes.
   Defined.
+
+  Context {orig_failure_params : FailureParams orig_multi_params}.
+
+  Instance serialized_failure_params : FailureParams serialized_multi_params :=
+    {
+      reboot := @reboot _ _ orig_failure_params
+    }.
+
+  Context {orig_name_overlay_params : NameOverlayParams orig_multi_params}.
+
+  Instance serialized_name_overlay_params : NameOverlayParams serialized_multi_params :=
+    {
+      adjacent_to := @adjacent_to _ _ orig_name_overlay_params;
+      adjacent_to_dec := @adjacent_to_dec _ _ orig_name_overlay_params;
+      adjacent_to_symmetric := @adjacent_to_symmetric _ _ orig_name_overlay_params;
+      adjacent_to_irreflexive := @adjacent_to_irreflexive _ _ orig_name_overlay_params
+    }.
+
+  Context {orig_fail_msg_params : FailMsgParams orig_multi_params}.
+
+  Instance serialized_fail_msg_params : FailMsgParams serialized_multi_params :=
+    {
+      msg_fail := serialize msg_fail
+    }.
+
+  Context {orig_new_msg_params : NewMsgParams orig_multi_params}.
+
+  Instance serialized_new_msg_params : NewMsgParams serialized_multi_params :=
+    {
+      msg_new := serialize msg_new
+    }.
 End Serialized.
 
-Hint Extern 5 (@BaseParams) => apply base_params : typeclass_instances.
-Hint Extern 5 (@MultiParams _) => apply multi_params : typeclass_instances.
+Hint Extern 5 (@BaseParams) => apply serialized_base_params : typeclass_instances.
+Hint Extern 5 (@MultiParams _) => apply serialized_multi_params : typeclass_instances.
+Hint Extern 5 (@FailureParams _ _) => apply serialized_failure_params : typeclass_instances.
